Add sequence neq lemma

Sequences/NatSeq.dfy
@@ -4,7 +4,7 @@ include "../NativeTypes.dfy"
 include "../Nonlinear_Arithmetic/Power.dfy"
 include "Seq.dfy"
 
-module IntSeq {
+abstract module NatSeq {
 
   import opened DivMod
   import opened Mul
@@ -12,8 +12,9 @@ module IntSeq {
   import opened Power
   import opened Seq
 
-  const BASE: int := BASE_32
-  type BaseType = i | 0 <= i < BASE
+  function method BASE(): nat
+		ensures BASE() > 1
+  type uint = i: int | 0 <= i < BASE()
 
   //////////////////////////////////////////////////////////////////////////////
   //
@@ -22,51 +23,51 @@ module IntSeq {
   //////////////////////////////////////////////////////////////////////////////
 
   /* Converts a sequence to nat. */
-  function method {:opaque} to_nat(xs: seq<BaseType>): nat
+  function method {:opaque} to_nat(xs: seq<uint>): nat
   {
     if |xs| == 0 then 0
     else
       lemma_power_positive_auto();
       lemma_mul_nonnegative_auto();
-      to_nat(drop_last(xs)) + last(xs) * power(BASE, |xs| - 1)
+      to_nat(drop_last(xs)) + last(xs) * power(BASE(), |xs| - 1)
   }
 
   /* Proves the nat representation of a sequence of length 1. */
-  lemma lemma_seq_len_1_nat(xs: seq<BaseType>)
+  lemma lemma_seq_len_1_nat(xs: seq<uint>)
     requires |xs| == 1
-    ensures to_nat(xs) == xs[0]
+    ensures to_nat(xs) == first(xs)
   {
     reveal to_nat();
     reveal power();
   }
 
   /* Proves the nat representation of a sequence of length 2. */
-  lemma lemma_seq_len_2_nat(xs: seq<BaseType>)
+  lemma lemma_seq_len_2_nat(xs: seq<uint>)
     requires |xs| == 2
-    ensures to_nat(xs) == xs[0] + xs[1] * BASE
+    ensures to_nat(xs) == first(xs) + xs[1] * BASE()
   {
     reveal to_nat();
     lemma_seq_len_1_nat(drop_last(xs));
     reveal power();
   }
 
-  lemma lemma_seq_equivalence(xs: seq<BaseType>, ys: seq<BaseType>)
+  lemma lemma_seq_equivalence(xs: seq<uint>, ys: seq<uint>)
     requires xs == ys
     ensures to_nat(xs) == to_nat(ys)
   {
     reveal to_nat();
   }
 
-  /* Proves the nat representation of a sequence is bounded by BASE to the
+  /* Proves the nat representation of a sequence is bounded by BASE() to the
   power of the sequence length. */
-  lemma lemma_seq_nat_bound(xs: seq<BaseType>)
-    ensures to_nat(xs) < power(BASE, |xs|)
+  lemma lemma_seq_nat_bound(xs: seq<uint>)
+    ensures to_nat(xs) < power(BASE(), |xs|)
   {
     reveal to_nat();
     reveal power();
     if |xs| != 0 {
       var len' := |xs| - 1;
-      var pow := power(BASE, len');
+      var pow := power(BASE(), len');
       calc {
         to_nat(xs);
         to_nat(drop_last(xs)) + last(xs) * pow;
@@ -74,67 +75,119 @@ module IntSeq {
         pow + last(xs) * pow;
         <=
           {
-            assert last(xs) <= BASE - 1;
+            assert last(xs) <= BASE() - 1;
             lemma_power_positive_auto();
             lemma_mul_inequality_auto();
           }
-        pow + (BASE - 1) * pow;
-        power(BASE, len' + 1);
+        pow + (BASE() - 1) * pow;
+          { lemma_mul_is_distributive_auto(); }
+        power(BASE(), len' + 1);
       }
     }
   }
 
-  function method {:opaque} prefix_nat(xs: seq<BaseType>, i: nat): nat
-    requires 0 <= i <= |xs|
+  lemma lemma_seq_inequality(xs: seq<uint>, ys: seq<uint>, i: nat)
+    requires 0 <= i < |xs| == |ys|
+    requires xs[i] < ys[i]
+    ensures to_nat(xs[..i+1]) < to_nat(ys[..i+1])
   {
-    to_nat(xs[..i])
-  }
-
-  lemma lemma_prefix_equivalence(xs: seq<BaseType>, ys: seq<BaseType>, i: nat)
-    requires 0 <= i <= |xs| && 0 <= i <= |ys|
-    requires xs[..i] == ys[..i]
-    ensures prefix_nat(xs, i) == prefix_nat(ys, i)
-  {
-    reveal prefix_nat();
-  }
-
-  /* Proves the nat representation of a prefix based on a smmaller prefix. */
-  lemma lemma_prefix_nat(xs: seq<BaseType>, i: nat)
-    requires 1 <= i < |xs|
-    ensures prefix_nat(xs, i)
-         == prefix_nat(xs, i - 1) + xs[i - 1] * power(BASE, i - 1)
-  {
-    assert xs[..i][..i-1] == xs[..i-1];
-    reveal prefix_nat();
     reveal to_nat();
+    calc {
+      to_nat(xs[..i+1]);
+      == { assert drop_last(xs[..i+1]) == xs[..i+1][..i] == xs[..i]; }
+      to_nat(xs[..i]) + xs[i] * power(BASE(), i);
+      < { lemma_seq_nat_bound(xs[..i]); }
+      power(BASE(), i) + xs[i] * power(BASE(), i);
+      == { lemma_mul_is_distributive_auto(); }
+      (1 + xs[i]) * power(BASE(), i);
+      <= { lemma_power_positive(BASE(), i); lemma_mul_inequality_auto(); }
+      ys[i] * power(BASE(), i);
+      <=
+      to_nat(ys[..i+1]);
+    }
+  }
+
+  lemma lemma_seq_neq_append(xs: seq<uint>, ys: seq<uint>, i: nat)
+    requires 0 <= i <= |xs| == |ys|
+    requires to_nat(xs[..i]) != to_nat(ys[..i])
+    ensures to_nat(xs) != to_nat(ys)
+    decreases |xs| - i
+  {
+    if i == |xs| {
+      assert xs[..i] == xs;
+      assert ys[..i] == ys;
+    } else {
+      reveal to_nat();
+      if xs[i] == ys[i] {
+        assert drop_last(xs[..i+1]) == xs[..i];
+        assert drop_last(ys[..i+1]) == ys[..i];
+      } else {
+        if xs[i] < ys[i]  { lemma_seq_inequality(xs, ys, i); }
+        else              { lemma_seq_inequality(ys, xs, i); }
+      }
+      lemma_seq_neq_append(xs, ys, i + 1);
+    }
+  }
+
+  lemma {:induction n} lemma_seq_neq(xs: seq<uint>, ys: seq<uint>, n: nat)
+    requires |xs| == |ys| == n
+    requires xs != ys
+    ensures to_nat(xs) != to_nat(ys)
+  {
+    ghost var i: nat := 0;
+
+    while i < n
+      invariant 0 <= i < n
+      invariant xs[..i] == ys[..i]
+    {
+      if xs[i] != ys[i] {
+        break;
+      }
+      i := i + 1;
+    }
+
+    reveal to_nat();
+    assert xs[..i+1][..i] == xs[..i];
+    lemma_seq_equivalence(drop_last(xs[..i+1]), drop_last(ys[..i+1]));
+    lemma_power_positive_auto();
+    lemma_mul_strict_inequality_auto();
+    assert to_nat(xs[..i+1]) != to_nat(ys[..i+1]);
+
+    lemma_seq_neq_append(xs, ys, i+1);
   }
 
   /* Proves mod equivalence between the nat representation of a sequence and
   the lsw of the sequence.*/
-  lemma lemma_seq_lsw_mod_equivalence(xs: seq<BaseType>)
+  lemma lemma_seq_lsw_mod_equivalence(xs: seq<uint>)
     requires |xs| >= 1;
-    ensures is_mod_equivalent(to_nat(xs), xs[0], BASE);
+    ensures is_mod_equivalent(to_nat(xs), first(xs), BASE());
   {
     if |xs| == 1 {
       lemma_seq_len_1_nat(xs);
+      lemma_mod_equivalence_auto();
     } else {
-      assert is_mod_equivalent(to_nat(xs), xs[0], BASE) by {
-        var len' := |xs| - 1;
-        var pow := power(BASE, len');
+      assert is_mod_equivalent(to_nat(xs), first(xs), BASE()) by {
+        var pow := power(BASE(), |xs| - 1);
         var xs' := drop_last(xs);
 
+        reveal to_nat();
         calc ==> {
           true;
-            { reveal to_nat(); }
-          is_mod_equivalent(to_nat(xs), to_nat(xs') + last(xs) * pow, BASE);
+            { lemma_mod_equivalence_auto(); }
+          is_mod_equivalent(to_nat(xs), to_nat(xs') + last(xs) * pow, BASE());
             {
+              lemma_mul_mod_noop_right_auto();
               lemma_power_mod_auto();
-              lemma_mul_mod_noop_general_auto();
-              assert is_mod_equivalent(last(xs) * pow, 0, BASE);
+              lemma_mul_basics_auto();
             }
-          is_mod_equivalent(to_nat(xs), to_nat(xs'), BASE);
-            { lemma_seq_lsw_mod_equivalence(xs'); }
-          is_mod_equivalent(to_nat(xs), xs[0], BASE);
+          is_mod_equivalent(to_nat(xs), to_nat(xs'), BASE());
+            {
+              lemma_seq_lsw_mod_equivalence(xs');
+              lemma_mod_equivalence(to_nat(xs), to_nat(xs'), BASE());
+              lemma_mod_equivalence(to_nat(xs'), first(xs'), BASE());
+              lemma_mod_equivalence(to_nat(xs), first(xs), BASE());
+            }
+          is_mod_equivalent(to_nat(xs), first(xs), BASE());
         }
       }
     }
@@ -147,13 +200,13 @@ module IntSeq {
   //////////////////////////////////////////////////////////////////////////////
 
   /* Converts a nat to a sequence. */
-  function method {:opaque} to_seq(x: nat): seq<BaseType>
-    decreases x
+  function method {:opaque} to_seq(x: nat): seq<uint>
   {
     if x == 0 then []
     else
       lemma_div_basics_auto();
-      to_seq(x / BASE) + [x % BASE]
+      lemma_div_decreases_auto();
+      to_seq(x / BASE()) + [x % BASE()]
   }
 
 
@@ -164,7 +217,7 @@ module IntSeq {
   //////////////////////////////////////////////////////////////////////////////
 
   /* Generates a sequence of zeros with length len. */
-  function method {:opaque} seq_zero(len: nat): (zs: seq<BaseType>)
+  function method {:opaque} seq_zero(len: nat): (zs: seq<uint>)
     ensures |zs| == len
   {
     if len == 0 then [] else seq_zero(len - 1) + [0]
@@ -180,7 +233,7 @@ module IntSeq {
         to_nat(seq_zero(len));
           { reveal seq_zero(); }
         to_nat(seq_zero(len - 1) + [0]);
-        to_nat(seq_zero(len - 1)) + 0 * power(BASE, len - 1);
+        to_nat(seq_zero(len - 1)) + 0 * power(BASE(), len - 1);
           {
             lemma_seq_zero_nat(len - 1);
             lemma_mul_basics_auto();
@@ -191,9 +244,9 @@ module IntSeq {
   }
 
   /* Adding a zero as the least significant bit is equal to multiplying the
-  number by BASE. */
-  lemma lemma_seq_prepend_zero(xs: seq<BaseType>)
-    ensures to_nat([0] + xs) == to_nat(xs) * BASE
+  number by BASE(). */
+  lemma lemma_seq_prepend_zero(xs: seq<uint>)
+    ensures to_nat([0] + xs) == to_nat(xs) * BASE()
   {
     reveal to_nat();
     if |xs| == 0 {
@@ -202,22 +255,22 @@ module IntSeq {
       calc {
         to_nat([0] + xs);
           { assert drop_last([0] + xs) == [0] + drop_last(xs); }
-        to_nat([0] + drop_last(xs)) + last(xs) * power(BASE, |xs|);
+        to_nat([0] + drop_last(xs)) + last(xs) * power(BASE(), |xs|);
           { lemma_seq_prepend_zero(drop_last(xs)); }
-        to_nat(drop_last(xs)) * BASE + last(xs) * power(BASE, |xs|);
+        to_nat(drop_last(xs)) * BASE() + last(xs) * power(BASE(), |xs|);
           {
             reveal power();
             lemma_mul_properties();
           }
-        (to_nat(drop_last(xs)) + last(xs) * power(BASE, |xs| - 1)) * BASE;
-        to_nat(xs) * BASE;
+        (to_nat(drop_last(xs)) + last(xs) * power(BASE(), |xs| - 1)) * BASE();
+        to_nat(xs) * BASE();
       }
     }
   }
 
   /* Adding zero(s) as the most significant bit(s) does not change the value of
   the number. */
-  lemma lemma_seq_append_zero(xs': seq<BaseType>, xs: seq<BaseType>) 
+  lemma lemma_seq_append_zero(xs': seq<uint>, xs: seq<uint>) 
     requires |xs'| < |xs|
     requires var len' := |xs'|;
       && drop_last(xs) == xs'
@@ -229,7 +282,7 @@ module IntSeq {
     if len != len' + 1 {
       calc == {
         to_nat(xs);
-        to_nat(drop_last(xs)) + last(xs) * power(BASE, len - 1);
+        to_nat(drop_last(xs)) + last(xs) * power(BASE(), len - 1);
         to_nat(drop_last(xs));
           { lemma_seq_append_zero(xs', drop_last(xs)); }
         to_nat(xs');
@@ -244,8 +297,8 @@ module IntSeq {
   //////////////////////////////////////////////////////////////////////////////
 
   /* Adds two sequences. */
-  function method {:opaque} seq_add(xs: seq<BaseType>,
-                                    ys: seq<BaseType>): (seq<BaseType>, nat)
+  function method {:opaque} seq_add(xs: seq<uint>,
+                                    ys: seq<uint>): (seq<uint>, nat)
     requires |xs| == |ys|
     ensures var (zs, cout) := seq_add(xs, ys); |zs| == |xs|
   {
@@ -254,19 +307,19 @@ module IntSeq {
     else
       var (zs', cin) := seq_add(drop_last(xs), drop_last(ys));
       var sum: int := last(xs) + last(ys) + cin;
-      var (sum_out, cout) := if sum < BASE then (sum, 0) else (sum - BASE, 1);
+      var (sum_out, cout) := if sum < BASE() then (sum, 0) else (sum - BASE(), 1);
       (zs' + [sum_out], cout)
   }
 
   /* Proves seq_add yields the same value as converting the sequences to nats,
   then adding them. */
-  lemma lemma_seq_add_nat(xs: seq<BaseType>,
-                          ys: seq<BaseType>,
-                          zs: seq<BaseType>,
+  lemma lemma_seq_add_nat(xs: seq<uint>,
+                          ys: seq<uint>,
+                          zs: seq<uint>,
                           cout: nat)
     requires |xs| == |ys|
     requires seq_add(xs, ys) == (zs, cout)
-    ensures to_nat(xs) + to_nat(ys) == to_nat(zs) + cout * power(BASE, |xs|)
+    ensures to_nat(xs) + to_nat(ys) == to_nat(zs) + cout * power(BASE(), |xs|)
   {
     reveal seq_add();
     reveal to_nat();
@@ -274,11 +327,11 @@ module IntSeq {
       reveal power();
     } else {
       var len' := |xs| - 1;
-      var pow := power(BASE, len');
+      var pow := power(BASE(), len');
       var (zs', cin) := seq_add(drop_last(xs), drop_last(ys));
       var sum: int := last(xs) + last(ys) + cin;
-      var z := if sum < BASE then sum else sum - BASE;
-      assert sum == z + cout * BASE;
+      var z := if sum < BASE() then sum else sum - BASE();
+      assert sum == z + cout * BASE();
 
       calc {
         to_nat(zs);
@@ -287,22 +340,22 @@ module IntSeq {
         to_nat(drop_last(xs)) + to_nat(drop_last(ys)) - cin * pow + z * pow;
           {
             lemma_mul_equality_auto();
-            assert sum * pow == (z + cout * BASE) * pow;
+            assert sum * pow == (z + cout * BASE()) * pow;
             lemma_mul_is_distributive_auto();
           } 
-        to_nat(xs) + to_nat(ys) - cout * BASE * pow;
+        to_nat(xs) + to_nat(ys) - cout * BASE() * pow;
           {
-            lemma_mul_is_associative(cout, BASE, pow);
+            lemma_mul_is_associative(cout, BASE(), pow);
             reveal power();
           }
-        to_nat(xs) + to_nat(ys) - cout * power(BASE, |xs|);
+        to_nat(xs) + to_nat(ys) - cout * power(BASE(), |xs|);
       }
     }
   }
 
   /* Subtracts two sequences. */
-  function method {:opaque} seq_sub(xs: seq<BaseType>,
-                                    ys: seq<BaseType>): (seq<BaseType>, nat)
+  function method {:opaque} seq_sub(xs: seq<uint>,
+                                    ys: seq<uint>): (seq<uint>, nat)
     requires |xs| == |ys|
     ensures var (zs, cout) := seq_sub(xs, ys); |zs| == |xs|
   {
@@ -312,19 +365,19 @@ module IntSeq {
       var (zs, cin) := seq_sub(drop_last(xs), drop_last(ys));
       var (diff_out, cout) := if last(xs) >= last(ys) + cin
                               then (last(xs) - last(ys) - cin, 0)
-                              else (BASE + last(xs) - last(ys) - cin, 1);
+                              else (BASE() + last(xs) - last(ys) - cin, 1);
       (zs + [diff_out], cout)
   }
 
   /* Proves seq_sub yields the same value as converting the sequences to nats,
   then subtracting them. */
-  lemma lemma_seq_sub_nat(xs: seq<BaseType>,
-                          ys: seq<BaseType>,
-                          zs: seq<BaseType>,
+  lemma lemma_seq_sub_nat(xs: seq<uint>,
+                          ys: seq<uint>,
+                          zs: seq<uint>,
                           cout: nat)
     requires |xs| == |ys|
     requires seq_sub(xs, ys) == (zs, cout)
-    ensures to_nat(xs) - to_nat(ys) + cout * power(BASE, |xs|) == to_nat(zs)
+    ensures to_nat(xs) - to_nat(ys) + cout * power(BASE(), |xs|) == to_nat(zs)
   {
     reveal seq_sub();
     reveal to_nat();
@@ -332,12 +385,12 @@ module IntSeq {
       reveal power();
     } else {
       var len' := |xs| - 1;
-      var pow := power(BASE, len');
+      var pow := power(BASE(), len');
       var (zs', cin) := seq_sub(drop_last(xs), drop_last(ys));
       var z := if last(xs) >= last(ys) + cin
                then last(xs) - last(ys) - cin
-               else BASE + last(xs) - last(ys) - cin;
-      assert cout * BASE + last(xs) - cin - last(ys) == z;
+               else BASE() + last(xs) - last(ys) - cin;
+      assert cout * BASE() + last(xs) - cin - last(ys) == z;
       
       calc {
         to_nat(zs);
@@ -346,15 +399,15 @@ module IntSeq {
         to_nat(drop_last(xs)) - to_nat(drop_last(ys)) + cin * pow + z * pow;
           {
             lemma_mul_equality_auto();
-            assert pow * (cout * BASE + last(xs) - cin - last(ys)) == pow * z;
+            assert pow * (cout * BASE() + last(xs) - cin - last(ys)) == pow * z;
             lemma_mul_is_distributive_auto();
           }
-        to_nat(xs) - to_nat(ys) + cout * BASE * pow;
+        to_nat(xs) - to_nat(ys) + cout * BASE() * pow;
           {
-            lemma_mul_is_associative(cout, BASE, pow);
+            lemma_mul_is_associative(cout, BASE(), pow);
             reveal power();
           }
-        to_nat(xs) - to_nat(ys) + cout * power(BASE, |xs|);
+        to_nat(xs) - to_nat(ys) + cout * power(BASE(), |xs|);
       }
     }
   }
